\def\duedate{September 5, 2023}
\def\HWnum{1}
\input{../preamble.tex}

\begin{document}

\prob{1}{
Calculate the series
\begin{eqnarray}
   I_1 = \sum_{n=1}^{\infty} \frac{1}{4^{n}}, \quad I_2 = \sum_{n=0}^{\infty} \frac{(-1)^{n}}{3^{n}}
.\end{eqnarray}
}

\sol{
Recall that for a geometric series $\sum_{n=0}^{\infty} a r^{n} = a/(1 - r)$.

For $I_1$, we can write
\begin{eqnarray}
    \eqbox{I_1 = \sum_{n=0}^{\infty} \frac{1}{4^{n}} - 1 = \frac{1}{1 - 1/4} - 1 = \frac{1}{3}}
.\end{eqnarray}

For $I_2$, $a = 1$ and $r = -1/3$, meaning $I_{2}$
\begin{eqnarray}
    \eqbox{I_{2} = \frac{1}{1 + 1/3} = \frac{3}{4}}
.\end{eqnarray}
}


\prob{2}{
Calculate the sum
\begin{eqnarray}
    I_3 = \sum_{n=1}^{N} \Big[ \frac{1}{n} - \frac{1}{1+n} \Big]
.\end{eqnarray}
What is the limit of $I_3$ at $N \rightarrow \infty$.
}

\sol{
We can split $I_3$ into two series as
\begin{eqnarray}
   I_3 = \sum_{n=1}^{N} \frac{1}{n} - \sum_{n=1}^{N} \frac{1}{n+1} 
,\end{eqnarray}
and we can shift indices on the second series with the substitution $m = n+1$ such that
\begin{eqnarray}
    \eqbox{I_3 = \sum_{n=1}^{N} \frac{1}{n} - \sum_{m=2}^{N+1} \frac{1}{m} = 1 - \frac{1}{N+1} = \frac{N}{N+1}}
.\end{eqnarray}
The infinite series
\begin{eqnarray}
    \eqbox{\lim_{N \rightarrow \infty} I_3 = \sum_{n=1}^{\infty} \Big[ \frac{1}{n} - \frac{1}{n+1} \Big] = 1}
\end{eqnarray}
since $1/(N+1) \rightarrow 0$ as $N \rightarrow \infty$
}


\prob{3}{
Does the alternating series
\begin{eqnarray}
   I_1 = \sum_{n=1}^{\infty} \frac{(-1)^{n}}{n^{7/6}}
\end{eqnarray}
converge absolutely?
}

\sol{
The series $I_1$ converges absolutely:
\begin{eqnarray}
    \sum_{n=1}^{\infty} \Big| \frac{(-1)^{n}}{n^{7/6}} \Big| = \sum_{n=1}^{\infty} \frac{1}{n^{7/6}} < \int_{1}^{\infty} \frac{\dd{x}}{x^{7/6}} = -6 x^{-1/6} \big|_{1}^{\infty} = 6
.\end{eqnarray}
Since the series is bounded above and below $I_1$ is absolutely convergent.
}


\prob{4}{
Does the series
\begin{eqnarray}
    I_2 = \sum_{n=1}^{\infty} \frac{x}{(nx + 1)[(n + 1)x + 1]}
\end{eqnarray}
with $x > 0$ converge uniformly?
}

\sol{

Notice that we can write the series as
\begin{eqnarray}
    I_{2} = \sum_{n=1}^{\infty} \Big[ \frac{1}{nx + 1} - \frac{1}{(n+1)x + 1} \Big] = \sum_{n=1}^{\infty} \frac{1}{nx + 1} - \sum_{n=1}^{\infty} \frac{1}{(n+1)x + 1}
,\end{eqnarray}
The $N^{\rm th}$ partial sum is given as
\begin{eqnarray}
    I_{2,N} = \sum_{n=1}^{N} \frac{1}{nx + 1} - \sum_{n=1}^{N} \frac{1}{(n+1)x + 1}
,\end{eqnarray}
and the second sum can be rewritten by shifting indices to $m = n+1$ such that it is clear that the partial sum is simply
\begin{eqnarray}
   I_{2,N} = \frac{1}{x + 1} - \frac{1}{(N+1)x + 1}
.\end{eqnarray}
Taking the limit $N \rightarrow \infty$, we find
\begin{eqnarray}
   \eqbox{I_{2} = \frac{1}{x+1}} 
.\end{eqnarray}
which is continuous on $x > 0$, implying that $I_{2}$ is uniformly convergent on $x > 0$.
}


\prob{5}{
Calculate the infinite product
\begin{eqnarray}
    I_3 = \prod_{n=1}^{\infty} \Big[ 1 + \frac{(-1)^{n}}{n+1} \Big]
.\end{eqnarray}

}

\sol{

We can heuristically solve this problem by writing the first several terms of the product:
\begin{eqnarray}
\begin{aligned}
    I_{3} &= \Big( 1 - \frac{1}{2} \Big) \Big( 1 + \frac{1}{3} \Big) \Big( 1 - \frac{1}{4} \Big) \Big( 1 + \frac{1}{5} \Big) \Big( 1 - \frac{1}{6} \Big) \cdots \\
          &= \frac{1}{2} \cdot \frac{4}{3} \cdot \frac{3}{4} \cdot \frac{6}{5} \cdot \frac{5}{6} \cdots = \eqbox{ \frac{1}{2} }
.\end{aligned}
\end{eqnarray}

More formally, we can write the product in terms of its even and odd terms as follows
\begin{eqnarray}
\begin{aligned}
    I_{3} &= \frac{1}{2} \prod_{k=1}^{\infty} \Big[ 1 + \frac{(-1)^{2k}}{2k + 1} \Big] \Big[ 1 + \frac{(-1)^{2k+1}}{(2k+1) + 1} \Big] \\
          &= \frac{1}{2} \prod_{k=1}^{\infty} \frac{2k + 2}{2k + 1} \cdot \frac{2k + 1}{2k + 2} = \frac{1}{2}
.\end{aligned}
\end{eqnarray}

}




\end{document}
