\def\duedate{\today}
\def\HWnum{12}
\input{../preamble.tex}

\begin{document}

\prob{1}{

Using the approach discussed in class, calculate the evolution of $n(x,t)$ along the $x$-axis $-\infty < x < \infty$ described by the diffusion equation
\begin{eqnarray}
    \pdv{n}{t} = \pdv[2]{n}{x}
\end{eqnarray}
with the boundary conditions $n(\pm \infty,t) = 0$ and the initial condition
\begin{eqnarray}
    n(x,0) = n_0 e^{-x^2/a^2}
.\end{eqnarray}

}

\sol{

The one-dimensional Green function for the diffusion equation (with $D = 1$) on the $x$-axis is
\begin{eqnarray}
    G(x-x',t) = \frac{1}{2 \sqrt{\pi t}} e^{-(x - x')^2/4t}
.\end{eqnarray}
The temperature distribution at an arbitrary time $t$ is then a spatial convolution of the Green's function with the initial shape of the temperature distribution at time $t = 0$:
\begin{eqnarray}
\eqbox{
\begin{aligned}
    n(x,t) &= \int_{-\infty}^{\infty} \dd{x'} G(x-x',t) n(x',0) = \frac{n_0}{2 \sqrt{\pi t}} \int_{-\infty}^{\infty} \dd{x'} e^{-(x-x')^2/4t} e^{-x'^2/a^2} \\
           &= \frac{n_0}{2 \sqrt{\pi t}} \Big( 2a \sqrt{\frac{\pi t}{a^2 + 4t}} e^{-x^2/(a^2 + 4t)} \Big) = \frac{n_0}{\sqrt{1 + 4t/a^2}} e^{-x^2/(a^2 + 4t)}
.\end{aligned}
}
\end{eqnarray}

}


\prob{2}{

The temperature of a planar surface at $x = 0$ changes periodically: $T(0,t) = T_0 + T_1 \cos{\omega t}$.
Using the Fourier transform in $t$, calculate the temperature $T(x,t)$ away from the heated surface at $x > 0$ by solving the thermal diffusion equation
\begin{eqnarray}
    \pdv{T}{t} = D \pdv[2]{T}{x}
\end{eqnarray}
with the boundary condition $T(0,t) = T_0 + T_1 \cos{\omega t}$ at $x = 0$ and $T(\infty,t) = T_0$ at $x = \infty$.

}

\sol{

First, let's define $u(x,t) = T(x,t) - T_0$.
It is clear that $u$ satisfies the same diffusion equation as $T$ but with the updated boundary conditions $u(0,t) = T_1 \cos{\omega t}$ and $u(\infty,t) = 0$.
As suggested, let's take the Fourier transform of the diffusion equation in time:
\begin{eqnarray}
    \int_{-\infty}^{\infty} \dd{t} e^{-i \omega' t} \pdv{u}{t} = i \omega \tilde{u}(x,\omega') = D \pdv[2]{\tilde{u}(x,\omega')}{x}
.\end{eqnarray}
We find then that
\begin{eqnarray}
\begin{aligned}
    \tilde{u}(x,\omega') &= A e^{\sqrt{-i \omega' / D} \, x} + B e^{-\sqrt{-i \omega' / D} \, x} \\
                        &= A e^{k'(1-i)x} + B e^{-k'(1-i)x} \\
                        &= A e^{-i k' x} e^{k' x} + B e^{i k' x} e^{-k' x}
,\end{aligned}
\end{eqnarray}
where we have defined $k' = \sqrt{\omega'/2D}$.
Notice that the boundary condition $u(\infty,t) = 0$ gives $\tilde{u}(\infty,t) = 0$, meaning that we must have $A = 0$.

Next, observe that the Fourier transform of $u(0,t) = T_1 \cos{\omega t} = \frac{T_1}{2} (e^{i \omega t} + e^{-i \omega t})$ is 
\begin{eqnarray}
    \tilde{u}(0,\omega') = \pi T_1[ \delta(\omega' - \omega) + \delta(\omega' + \omega) ] = B
\end{eqnarray}
Thus,
\begin{eqnarray}
    \tilde{u}(x,\omega') = \pi T_1 [ \delta(\omega' - \omega) + \delta(\omega' + \omega) ] e^{i k' x} e^{-k'x}
.\end{eqnarray}

With this, we take the inverse Fourier transform of $\tilde{u}$ and find
\begin{eqnarray}
\begin{aligned}
    u(x,t) &= \frac{T_1}{2} \int_{-\infty}^{\infty} \dd{\omega'} e^{i \omega' t} [ \delta(\omega' - \omega) + \delta(\omega' + \omega) ] e^{(-1 + i) \sqrt{\omega'/2D} \, x} \\
           &= \frac{T_1}{2} \Big[ e^{i \omega t} e^{(-1+i)\sqrt{\omega/2D} \, x} + e^{-i \omega t} e^{-(1 + i)\sqrt{\omega/2D} \, x} \Big] \\
           &= T_1 \cos\Bigg[ \omega \Bigg( t + \frac{x}{\sqrt{2\omega D}} \Bigg) \Bigg] e^{-\sqrt{\omega / 2D} \, x}
.\end{aligned}
\end{eqnarray}

Finally, we add $T_0$ to $u$ and arrive at
\begin{eqnarray}
    \eqbox{ T(x,t) = T_0 + T_1 \cos\Bigg[ \omega \Bigg( t + \frac{x}{\sqrt{2\omega D}} \Bigg) \Bigg] \exp( - \sqrt{\frac{\omega}{2D}} \, x ) }
.\end{eqnarray}


}




\end{document}
