\def\duedate{\today}
\def\HWnum{2}
\input{../preamble.tex}

\begin{document}

\prob{1}{

Calculate the following limit:
\begin{eqnarray}
    I_{1} = \lim_{x \rightarrow 0} \frac{x^2 \ln(1 + x^2)}{x^2 - \sin^2{x}}
.\end{eqnarray}

}

\sol{

Upon first glance, we have a limit of an indeterminate form $0/0$.
We may use L'Hopital's rule, but the functions are quite messy to differentiate, so we expand both the numerator and denominator in Taylor series about $x = 0$.
Note that $\ln(1 + x) = x - x^2/2 + {\rm cal O}(x^3)$ and $\sin^2{x} = (1 - \cos{2x})/2 = [(2x)^2/2! + (2x)^{4}/4! + {\cal O}(x^{6})]/2$.
Thus, the limit
\begin{eqnarray}
    \eqbox{ I_{1} = \lim_{x \rightarrow 0} \frac{ x^{4} }{ x^2 - \frac{1}{2}[(2x)^2/2! - (2x)^{4}/4!] } = \frac{2(4!)}{2^{4}} = \frac{24}{8} = 3 }
.\end{eqnarray}


}


\prob{2}{

Calculate the following limit of the $m-{\rm th}$ derivative at $x = 0$:
\begin{eqnarray}
    I_{2} = \lim_{x \rightarrow 0} \dv[m]{x} \frac{\ln(1 + x) - x}{x^2}
.\end{eqnarray}

}

\sol{

Here, we can write
\begin{eqnarray}
    \begin{aligned}
        \frac{\ln(1 + x) - x}{x^2} &= \frac{1}{x^2} \Big[ \sum_{n=1}^{\infty} \frac{(-1)^{n+1} x^{n}}{n} - x \Big] = \sum_{n=2}^{\infty} \frac{(-1)^{n+1}}{n} x^{n-2} = \sum_{n=0}^{\infty} \frac{(-1)^{n+1}}{n+2} x^{n} \\
                                   &= \sum_{n=0}^{m-1} \frac{(-1)^{n+1}}{n+2} x^{n} + \frac{(-1)^{m+1}}{m+2} x^{m} + \sum_{n=m+1} \frac{(-1)^{n+1}}{n+2} x^{n}
    .\end{aligned}
\end{eqnarray}
The last step is mostly illustrative for this:
\begin{eqnarray}
    \dv[m]{x} \frac{\ln(1 + x) - x}{x^2} = \frac{(-1)^{m+1} \, m!}{m+2} + {\cal O}(x)
.\end{eqnarray}
Therefore, taking $x \rightarrow 0$ gives
\begin{eqnarray}
    \eqbox{ I_{2} = (-1)^{m+1} \frac{m!}{m+2} }
.\end{eqnarray}


}


\prob{3}{

Calculate the following limit at $x = y = 0$:
\begin{eqnarray}
    I_{3} = \lim_{x \rightarrow 0, y \rightarrow 0} \laplacian \big[ e^{-ax^2 - by^2} \cos{ax} \cos{by} \big]
.\end{eqnarray}

}

\sol{

We can rewrite the operand of the laplacian as
\begin{eqnarray}
    e^{-ax^2-by^2} \cos{ax} \cos{by} = [e^{-ax^2}\cos{ax}] [e^{-by^2} \cos{bx}]
,\end{eqnarray}
which gives
\begin{eqnarray}
    \laplacian e^{-ax^2 - by^2} \cos{ax} \cos{by} = e^{-by^2} \cos{by} \pdv[2]{x} e^{-ax^2} \cos{ax} + e^{-ax^2} \cos{ax} \pdv[2]{y} e^{-by^2} \cos{by}
.\end{eqnarray}
Note that we can evaluate the limit of the first term and use the replacements $a \leftrightarrow b,~ x \leftrightarrow y$.

Observe that
\begin{eqnarray}
    \lim_{y \rightarrow 0} e^{-b y^2} \cos{b y} = 1
.\end{eqnarray}
Next, we evaluate the second factor to be
\begin{eqnarray}
    \begin{aligned}
        \dv[2]{x} e^{-ax^2} \cos{ax} &= -2a (1 - 2ax) e^{-ax^2} \cos{ax} + (- 2 a x e^{-ax^2})(-a \sin{ax}) \\
                                     &+ e^{-a x^2} (-a^2 \cos{ax})
    .\end{aligned}
\end{eqnarray}
It should be clear then that
\begin{eqnarray}
    \lim_{x \rightarrow 0} \pdv[2]{x} e^{-ax^2} \cos{ax} = -2a - a^2 = -(a + 1)^2 + 1 
.\end{eqnarray}
Hence 
\begin{eqnarray}
    \eqbox{ \lim_{x,y \rightarrow 0} \laplacian e^{-ax^2 - by^2} \cos{ax} \cos{by} = -(a + 1)^2 - (b + 1)^2 + 2 }
.\end{eqnarray}



}


\prob{4}{

Calculate the sum
\begin{eqnarray}
   I_{1} = \sum_{n=1}^{N} (n^2 + n + 1) 
.\end{eqnarray}

}

\sol{

We can use the Euler-Maclaurin formula 
\begin{eqnarray}
    \sum_{n=a}^{N} f(n) = \int_{a}^{N} f(x) \dd{x} + \frac{1}{2}[f(N) + f(a)] + \sum_{n=1}^{q} \frac{B_{2n}}{(2n)!}[ f^{(2n-1)}(N) - f^{(2n-1)}(a) ] + R
.\end{eqnarray}

to compute this series.
First, we split the sum into separate terms as
\begin{eqnarray}
    \label{eq:I1-parts}
    I_{1} = \sum_{n=0}^{N} n^2 + \sum_{n=0}^{N} n + N
,\end{eqnarray}
where we have gone ahead and evaluated the sum of the last term since it is just $1$ added $N$ times.
Also note that we have adjusted out indices to start from $n=0$ since this does not change the sum but should make the right hand side simpler to evaluate since $\dv[n]{x} x^{m}|_{x = 0} = 0$ for any $n,m \in \mathbb{N} \cup \{ 0 \}$.
The first sum is
\begin{eqnarray}
    \begin{aligned}
    \sum_{n=0}^{N} n^2 &= \int_{0}^{N} x^2 \dd{x} + \frac{N^2}{2} + \frac{B_{2}}{2!}\dv{x} (x^2)|_{x = N} = \frac{N^3}{3} + \frac{N^2}{2} + \frac{N}{6} \\
        &= \frac{N}{6}(2N^2 + 3N + 1) = \frac{N(N+1)(2N+1)}{6}
    \end{aligned}
.\end{eqnarray}
Moving on to the second sum we find\footnote{As Gauss did in his primary years using a much simpler and elegant rationale.}
\begin{eqnarray}
    \sum_{n=0}^{N} n = \int_{0}^{N} x \dd{x} + \frac{N}{2} = \frac{N^2}{2} + \frac{N}{2} = \frac{N(N+1)}{2}
.\end{eqnarray}

Plugging these intermediate results into \eref{I1-parts}, we find
\begin{eqnarray}
    \begin{aligned}
        I_{1} &= \frac{N(N+1)(2N+1)}{6} + \frac{N(N+1)}{2} + N \\
        &= \frac{N}{6} \Big[ (N+1) \Big( (2N+1) + 3 \Big) + 6 \Big] = \eqbox{ \frac{N(N^2 + 3N + 5)}{3} }
    .\end{aligned} 
\end{eqnarray}


}

\prob{5}{

Calculate the sum
\begin{eqnarray}
   I_2 = \sum_{n=1}^{\infty} \frac{(-1)^{n}}{n^2 + a^2} 
.\end{eqnarray}

}

\sol{

For this problem we can use the Poisson summation formula
\begin{eqnarray}
    \sum_{n=0}^{\infty} \frac{(-1)^{n}}{n^2 + a^2} = \int_{0}^{\infty} f(x) \dd{x} + \frac{f(0)}{2} + 2 \sum_{n=1}^{\infty} \int_{0}^{\infty} f(x) \cos{(2 \pi n x)} \dd{x}
.\end{eqnarray}
Note here that we can rewrite $(-1)^{n} = \cos{n \pi}$.
Using this, we find
\begin{eqnarray}
    \int_{0}^{\infty} \frac{\cos{k x}}{x^2 + a^2} \dd{x} = \frac{\pi}{2 |a|} e^{-k |a|}
.\end{eqnarray}
The sum is then given as
\begin{eqnarray}
    \begin{aligned}
        \sum_{n=0}^{\infty} \frac{(-1)^{n}}{n^2 + a^2} &= \frac{\pi}{2 |a|} e^{- \pi |a|} + \frac{1}{2a^2} + \sum_{n=1}^{\infty} \int_{0}^{\infty} \frac{\cos{[(2n+1)\pi x]} + \cos{[(2n - 1)\pi x]}}{n^2 + a^2} \dd{x} \\
        &= \frac{\pi}{2|a|}e^{- \pi |a|} +\frac{1}{2 a^2} + \sum_{n=1}^{\infty} \frac{\pi}{2 |a|} \Big[ e^{-(2n+1) \pi |a|}  + e^{-(2n - 1) \pi |a|} \Big] \\
        &= \frac{\pi}{2 |a|} e^{-\pi |a|} + \frac{1}{2 a^2} + \frac{\pi}{2|a|} \Big[ e^{-\pi|a|} \sum_{n=1}^{\infty} e^{-2n\pi|a|} + e^{\pi |a|} \sum_{n=1}^{\infty} e^{-2n\pi|a|} \Big] \\
        &= \frac{\pi}{2 |a|} e^{-\pi |a|} + \frac{1}{2 a^2} + \frac{\pi}{|a|} \cosh{\pi |a|} \frac{e^{-2 \pi |a|}}{1 - e^{-2 \pi |a|}} \\
        &= \frac{1}{2a^2} + \frac{\pi}{2|a|} e^{-\pi |a|} \Big[ 1 + \coth{\pi |a|} \Big]
    .\end{aligned}
\end{eqnarray}
At this point, we can subtract the $n=0$ term from both sides of the previous equation and obtain
\begin{eqnarray}
    \eqbox{ I_{2} = \sum_{n=0}^{\infty} \frac{(-1)^{n}}{n^2 + a^2} - \frac{1}{a^2} = -\frac{1}{2 a^2} + \frac{\pi}{2 |a|} e^{-\pi |a|} \Big[ 1 + \coth{\pi |a|} \Big] }
.\end{eqnarray}

}


\prob{6}{

Calculate the asymptotic series for this integral at $x \gg 1$:
\begin{eqnarray}
    I_{3} = \int_{x}^{\infty} e^{-au} \ln{u} \dd{u}
,\end{eqnarray}
where $a > 0$.

}

\sol{

We can solve this problem using integration by parts $\int f' g \dd{x} = fg - \int f g' \dd{x}$ with $f' = e^{-au}$ and $g = \ln{u}$, which gives $f = -\frac{1}{a}e^{-au} = -\frac{1}{a} f'$ and $g' = 1/u$.
Plugging this in, we find
\begin{eqnarray}
    I_{3} = -\frac{1}{a} \frac{e^{-au}}{u} \Big|_{x}^{\infty} + \frac{1}{a} \int_{x}^{\infty} \frac{e^{-au}}{u} \dd{u} = \frac{e^{-ax}}{ax} + \int_{x}^{\infty} \frac{e^{-au}}{au} \dd{u} = \frac{e^{-ax}}{ax} + \frac{1}{a} E_{1}(ax)
.\end{eqnarray}
Thus, we have
\begin{eqnarray}
    \eqbox{ I_{3} = \frac{e^{-ax}}{ax} + \frac{1}{a} e^{-ax} \sum_{n=0}^{\infty} \frac{(-1)^{n}}{(ax)^{n+1}} n! = \frac{e^{-ax}}{ax} \Bigg[ 1 + x \sum_{n=0}^{\infty} \frac{(-1)^{n}}{(ax)^{n+1}} n! \Bigg] }
.\end{eqnarray}


}



\end{document}
